src/goose_lang/ffi/async_disk_prelude.v
@@ -1,6 +1,6 @@
 From Perennial.goose_lang Require Import lang.
 From Perennial.goose_lang Require Export ffi.async_disk_proph.
-Existing Instances async_disk_proph.disk_op async_disk_proph.disk_model async_disk_proph.disk_ty.
+Existing Instances async_disk_syntax.disk_op async_disk_proph.disk_model async_disk_syntax.disk_ty.
 Existing Instances async_disk_proph.disk_semantics async_disk_proph.disk_interp.
 Existing Instance goose_diskGS.
 (* Now that the TC parameter is fixed, we can make this a coercion. *)
@@ -8,7 +8,7 @@ Coercion Var' (s: string) := Var s.
 
 
 Module disk.
-  Notation Disk := async_disk_proph.Disk.
+  Notation Disk := async_disk_syntax.Disk.
   Notation Write := async_disk_proph.Write.
   Notation Read := async_disk_proph.Read.
   Notation ReadTo := async_disk_proph.ReadTo.
@@ -16,7 +16,7 @@ Module disk.
 End disk.
 
 Module async_disk.
-  Notation BlockSize := async_disk_proph.BlockSize.
+  Notation BlockSize := async_disk_syntax.BlockSize.
   Notation Write := async_disk_proph.Write.
   Notation Read := async_disk_proph.Read.
   Notation ReadTo := async_disk_proph.ReadTo.
