src/goose_lang/ffi/async_disk_syntax.v
@@ -1,0 +1,71 @@
+From stdpp Require Import gmap.
+From stdpp Require Import vector fin_maps.
+From RecordUpdate Require Import RecordSet.
+From iris.algebra Require Import numbers.
+From Perennial.algebra Require Import gen_heap_names.
+From iris.proofmode Require Import tactics.
+From Perennial.program_logic Require Import ectx_lifting.
+
+From Perennial.Helpers Require Import CountableTactics Transitions.
+From Perennial.goose_lang Require Import lang lifting slice typing.
+From Perennial.goose_lang Require Import crash_modality.
+
+Set Default Proof Using "Type".
+(* this is purely cosmetic but it makes printing line up with how the code is
+usually written *)
+Set Printing Projections.
+
+Inductive DiskOp := ReadOp | WriteOp | SizeOp | BarrierOp.
+Instance eq_DiskOp : EqDecision DiskOp.
+Proof.
+  solve_decision.
+Defined.
+
+Instance DiskOp_fin : Countable DiskOp.
+Proof.
+  solve_countable DiskOp_rec 4%nat.
+Qed.
+
+Definition disk_op : ffi_syntax.
+Proof.
+  refine (mkExtOp DiskOp _ _ () _ _).
+Defined.
+
+Inductive Disk_ty := | DiskInterfaceTy.
+
+Instance disk_val_ty: val_types :=
+  {| ext_tys := Disk_ty; |}.
+
+Section disk.
+  Existing Instances disk_op disk_val_ty.
+
+  Inductive disk_ext_tys : @val disk_op -> (ty * ty) -> Prop :=
+  | DiskOpType op :
+      disk_ext_tys (λ: "v", ExternalOp op (Var "v"))%V
+                   (match op with
+                   | ReadOp => (uint64T, arrayT byteT)
+                   | WriteOp => (prodT uint64T (arrayT byteT), unitT)
+                   | SizeOp => (unitT, uint64T)
+                   | BarrierOp => (unitT, unitT)
+                   end).
+
+  Definition disk_ty: ext_types disk_op :=
+    {| val_tys := disk_val_ty;
+       get_ext_tys := disk_ext_tys |}.
+  Definition Disk: ty := extT DiskInterfaceTy.
+End disk.
+
+Definition block_bytes: nat := Z.to_nat 4096.
+Definition BlockSize {ext: ffi_syntax}: val := #4096.
+Definition Block := vec byte block_bytes.
+Definition blockT `{ext_tys:ext_types}: @ty val_tys := slice.T byteT.
+(* TODO: could use vreplicate; not sure how much easier it is to work with *)
+Definition block0 : Block := list_to_vec (replicate (Z.to_nat 4096) (U8 0)).
+
+
+Lemma block_bytes_eq : block_bytes = Z.to_nat 4096.
+Proof. reflexivity. Qed.
+
+Global Instance Block0: Inhabited Block := _.
+Global Instance Block_countable : Countable Block := _.
+
